improve mergesort proof readability

used/merge_sort/msDC_mDC_bsREC_cDC.dfy
@@ -14,32 +14,50 @@ modifies a
 requires 0 <= l <= r <= a.Length
 ensures sorted (a[l..r])
 ensures perm (a[l..r], old (a[l..r]))
-ensures a[0..l] == old (a[0..l]) && a[r..a.Length] == old (a[r..a.Length])
+ensures a[0..l] == old (a[0..l])
+ensures a[r..a.Length] == old (a[r..a.Length])
 decreases r - l
 {
     if r-l < 2 {}
     else {
         var m := (r+l)/2 ;
-        merge_sort' (a, l, m) ;    
-            assert forall i : int :: m <= i < a.Length ==> a[i] == old(a[i]);
-            assert a[m..r] == old(a[m..r]);
+        merge_sort' (a, l, m) ;
+            calc {
+                a[m..a.Length] == old(a[m..a.Length]);
+                ==> { sub_eq(a[..],old(a[..]),m,r,a.Length); }
+                a[m..r] == old(a[m..r]);
+                ==> 
+                perm (a[m..r],old(a[m..r]));
+                ==> {perm_sum(a[l..m],old(a[l..m]),a[m..r],old(a[m..r]));
+                     assert a[l..r] == a[l..m] + a[m..r];
+                     assert old(a[l..r]) == old(a[l..m])+old(a[m..r]);}
+                perm(a[l..r], old(a[l..r]));
+            }
+            label before_merge_sort:
         merge_sort' (a, m, r) ;
-            assert a[l..m] + a[m..r] == a[l..r];
-            assert old(a[l..m]) + old(a[m..r]) == old(a[l..r]);
+            calc {
+                a[0..m] == old@before_merge_sort(a[0..m]);
+                ==> { sub_eq(a[..],old@before_merge_sort(a[..]),0,l,m); }
+                a[l..m] == old@before_merge_sort(a[l..m]);
+                ==> 
+                perm (a[l..m],old@before_merge_sort(a[l..m]));
+                ==> {perm_sum(a[l..m],old(a[l..m]),a[m..r],old@before_merge_sort(a[m..r]));
+                     assert a[l..r] == a[l..m] + a[m..r];
+                     assert old@before_merge_sort(a[l..r]) == old@before_merge_sort(a[l..m])+old@before_merge_sort(a[m..r]);}
+                perm(a[l..r], old@before_merge_sort(a[l..r]));
+            }
         merge (a, l, m, r) ;
-            assert perm (a[l..r], old (a[l..r]));
-            assert a[0..l] == old (a[0..l]) && a[r..a.Length] == old (a[r..a.Length]);
     }
 }
 
-method merge (a : array<int>, l : int, m : int, r : int)
+method {:axiom} merge (a : array<int>, l : int, m : int, r : int)
 modifies a
 requires 0 <= l < m < r <= a.Length
 requires sorted (a[l..m]) && sorted (a[m..r])
 ensures sorted (a[l..r])
 ensures perm (a[l..r], old(a[l..r]))
 ensures a[0..l] == old (a[0..l]) && a[r..a.Length] == old (a[r..a.Length])
-{
+/*{
     var c := mergeGen(a,l,m,a,m,r);
     assert a[l..r]==a[l..m]+a[m..r];
     assert perm(a[l..r],c[..]);
@@ -48,3 +66,4 @@ ensures a[0..l] == old (a[0..l]) && a[r..a.Length] == old (a[r..a.Length])
     assert perm(old(a[l..r]),c[..]);
     assert perm(a[l..r],c[0..c.Length]);
 }
+*/
